<?xml version="1.0"?>
<rdf:RDF xmlns="http://purl.obolibrary.org/obo/uo.owl#"
     xml:base="http://purl.obolibrary.org/obo/uo.owl"
     xmlns:owl="http://www.w3.org/2002/07/owl#"
     xmlns:rdf="http://www.w3.org/1999/02/22-rdf-syntax-ns#"
     xmlns:xml="http://www.w3.org/XML/1998/namespace"
     xmlns:xsd="http://www.w3.org/2001/XMLSchema#"
     xmlns:rdfs="http://www.w3.org/2000/01/rdf-schema#"
     xmlns:oboInOwl="http://www.geneontology.org/formats/oboInOwl#">
    <owl:Ontology rdf:about="http://purl.obolibrary.org/obo/uo.owl">
        <owl:versionIRI rdf:resource="http://purl.obolibrary.org/obo/uo/releases/2023-05-25/uo.owl"/>
    </owl:Ontology>
    


    <!-- 
    ///////////////////////////////////////////////////////////////////////////////////////
    //
    // Annotation properties
    //
    ///////////////////////////////////////////////////////////////////////////////////////
     -->

    


    <!-- http://www.geneontology.org/formats/oboInOwl#hasExactSynonym -->

    <owl:AnnotationProperty rdf:about="http://www.geneontology.org/formats/oboInOwl#hasExactSynonym"/>
    


    <!-- http://www.geneontology.org/formats/oboInOwl#hasRelatedSynonym -->

    <owl:AnnotationProperty rdf:about="http://www.geneontology.org/formats/oboInOwl#hasRelatedSynonym"/>
    


    <!-- http://www.w3.org/2000/01/rdf-schema#comment -->

    <owl:AnnotationProperty rdf:about="http://www.w3.org/2000/01/rdf-schema#comment"/>
    


    <!-- http://www.w3.org/2000/01/rdf-schema#label -->

    <owl:AnnotationProperty rdf:about="http://www.w3.org/2000/01/rdf-schema#label"/>
    


    <!-- 
    ///////////////////////////////////////////////////////////////////////////////////////
    //
    // Classes
    //
    ///////////////////////////////////////////////////////////////////////////////////////
     -->

    


    <!-- http://purl.obolibrary.org/obo/UO_0000000 -->

    <owl:Class rdf:about="http://purl.obolibrary.org/obo/UO_0000000">
        <rdfs:subClassOf rdf:resource="http://www.w3.org/2002/07/owl#Thing"/>
        <rdfs:comment>&quot;A unit of measurement is a standardized quantity of a physical quality.&quot; [Wikipedia:Wikipedia]</rdfs:comment>
        <rdfs:label>unit</rdfs:label>
    </owl:Class>
    


    <!-- http://purl.obolibrary.org/obo/UO_0000001 -->

    <owl:Class rdf:about="http://purl.obolibrary.org/obo/UO_0000001">
        <rdfs:subClassOf rdf:resource="http://purl.obolibrary.org/obo/UO_0000000"/>
        <rdfs:comment>&quot;A unit which is a standard measure of the distance between two points.&quot; [Wikipedia:Wikipedia]</rdfs:comment>
        <rdfs:label>length unit</rdfs:label>
    </owl:Class>
    


    <!-- http://purl.obolibrary.org/obo/UO_0000002 -->

    <owl:Class rdf:about="http://purl.obolibrary.org/obo/UO_0000002">
        <rdfs:subClassOf rdf:resource="http://purl.obolibrary.org/obo/UO_0000000"/>
        <rdfs:comment>&quot;A unit which is a standard measure of the amount of matter/energy of a physical object.&quot; [Wikipedia:Wikipedia]</rdfs:comment>
        <rdfs:label>mass unit</rdfs:label>
    </owl:Class>
    


    <!-- http://purl.obolibrary.org/obo/UO_0000003 -->

    <owl:Class rdf:about="http://purl.obolibrary.org/obo/UO_0000003">
        <rdfs:subClassOf rdf:resource="http://purl.obolibrary.org/obo/UO_0000000"/>
        <oboInOwl:hasExactSynonym>time derived unit</oboInOwl:hasExactSynonym>
        <rdfs:comment>&quot;A unit which is a standard measure of the dimension in which events occur in sequence.&quot; [Wikipedia:Wikipedia]</rdfs:comment>
        <rdfs:label>time unit</rdfs:label>
    </owl:Class>
    


    <!-- http://purl.obolibrary.org/obo/UO_0000019 -->

    <owl:Class rdf:about="http://purl.obolibrary.org/obo/UO_0000019">
        <rdfs:subClassOf rdf:resource="http://purl.obolibrary.org/obo/UO_1000019"/>
        <oboInOwl:hasExactSynonym>Ã…</oboInOwl:hasExactSynonym>
        <rdfs:comment>&quot;A length unit which is equal to 10 [-10] m.&quot; [NIST:NIST]</rdfs:comment>
        <rdfs:label>angstrom</rdfs:label>
    </owl:Class>
    


    <!-- http://purl.obolibrary.org/obo/UO_0000030 -->

    <owl:Class rdf:about="http://purl.obolibrary.org/obo/UO_0000030">
        <rdfs:subClassOf rdf:resource="http://purl.obolibrary.org/obo/UO_1000010"/>
        <oboInOwl:hasExactSynonym>ps</oboInOwl:hasExactSynonym>
        <rdfs:comment>&quot;A time unit which is equal to 10^[-12] s.&quot; [NIST:NIST]</rdfs:comment>
        <rdfs:label>picosecond</rdfs:label>
    </owl:Class>
    


    <!-- http://purl.obolibrary.org/obo/UO_0000047 -->

    <owl:Class rdf:about="http://purl.obolibrary.org/obo/UO_0000047">
        <rdfs:subClassOf rdf:resource="http://purl.obolibrary.org/obo/UO_0000000"/>
        <rdfs:comment>&quot;A unit which is a standard measure of the amount of a 2-dimensional flat surface.&quot; [UOC:GVG]</rdfs:comment>
        <rdfs:label>area unit</rdfs:label>
    </owl:Class>
    


    <!-- http://purl.obolibrary.org/obo/UO_0000051 -->

    <owl:Class rdf:about="http://purl.obolibrary.org/obo/UO_0000051">
        <rdfs:subClassOf rdf:resource="http://purl.obolibrary.org/obo/UO_0000000"/>
        <rdfs:comment>&quot;A unit which represents a standard measurement of how much of a given substance there is mixed with another substance.&quot; [UOC:GVG]</rdfs:comment>
        <rdfs:label>concentration unit</rdfs:label>
    </owl:Class>
    


    <!-- http://purl.obolibrary.org/obo/UO_0000060 -->

    <owl:Class rdf:about="http://purl.obolibrary.org/obo/UO_0000060">
        <rdfs:subClassOf rdf:resource="http://purl.obolibrary.org/obo/UO_0000000"/>
        <rdfs:comment>&quot;A unit which is a standard measure of the rate of movement. Speed is measured in the same physical units of measurement as velocity, but does not contain the element of direction that velocity has. Speed is thus the magnitude component of velocity.&quot; [Wikipedia:Wikipedia]</rdfs:comment>
        <rdfs:label>speed/velocity unit</rdfs:label>
    </owl:Class>
    


    <!-- http://purl.obolibrary.org/obo/UO_0000061 -->

    <owl:Class rdf:about="http://purl.obolibrary.org/obo/UO_0000061">
        <rdfs:subClassOf rdf:resource="http://purl.obolibrary.org/obo/UO_0000051"/>
        <rdfs:comment>&quot;A concentration unit which is a standard measure of the number of moles of a given substance per liter of solution.&quot; [UOC:GVG]</rdfs:comment>
        <rdfs:label>unit of molarity</rdfs:label>
    </owl:Class>
    


    <!-- http://purl.obolibrary.org/obo/UO_0000062 -->

    <owl:Class rdf:about="http://purl.obolibrary.org/obo/UO_0000062">
        <rdfs:subClassOf rdf:resource="http://purl.obolibrary.org/obo/UO_1000062"/>
        <oboInOwl:hasExactSynonym>M</oboInOwl:hasExactSynonym>
        <rdfs:comment>&quot;A unit of concentration which expresses a concentration of 1 mole of solute per liter of solution (mol/L).&quot; [UOC:GVG]</rdfs:comment>
        <rdfs:label>molar</rdfs:label>
    </owl:Class>
    


    <!-- http://purl.obolibrary.org/obo/UO_0000063 -->

    <owl:Class rdf:about="http://purl.obolibrary.org/obo/UO_0000063">
        <rdfs:subClassOf rdf:resource="http://purl.obolibrary.org/obo/UO_1000062"/>
        <oboInOwl:hasExactSynonym>mM</oboInOwl:hasExactSynonym>
        <rdfs:comment>&quot;A unit of molarity which is equal to one thousandth of a molar or 10^[-3] M.&quot; [UOC:GVG]</rdfs:comment>
        <rdfs:label>millimolar</rdfs:label>
    </owl:Class>
    


    <!-- http://purl.obolibrary.org/obo/UO_0000094 -->

    <owl:Class rdf:about="http://purl.obolibrary.org/obo/UO_0000094">
        <rdfs:subClassOf rdf:resource="http://purl.obolibrary.org/obo/UO_1000094"/>
        <oboInOwl:hasExactSynonym>m/s</oboInOwl:hasExactSynonym>
        <oboInOwl:hasExactSynonym>metre per second</oboInOwl:hasExactSynonym>
        <rdfs:comment>&quot;A speed/velocity unit which is equal to the speed of an object traveling 1 meter distance in one second.&quot; [NIST:NIST]</rdfs:comment>
        <rdfs:label>meter per second</rdfs:label>
    </owl:Class>
    


    <!-- http://purl.obolibrary.org/obo/UO_0000105 -->

    <owl:Class rdf:about="http://purl.obolibrary.org/obo/UO_0000105">
        <rdfs:subClassOf rdf:resource="http://purl.obolibrary.org/obo/UO_0000000"/>
        <rdfs:comment>&quot;A unit which is a standard measure of the number of repetitive actions in a particular time.&quot; [NIST:NIST]</rdfs:comment>
        <rdfs:label>frequency unit</rdfs:label>
    </owl:Class>
    


    <!-- http://purl.obolibrary.org/obo/UO_0000109 -->

    <owl:Class rdf:about="http://purl.obolibrary.org/obo/UO_0000109">
        <rdfs:subClassOf rdf:resource="http://purl.obolibrary.org/obo/UO_0000000"/>
        <rdfs:comment>&quot;A unit which is a standard measure of the force applied to a given area.&quot; [NIST:NIST]</rdfs:comment>
        <rdfs:label>pressure unit</rdfs:label>
    </owl:Class>
    


    <!-- http://purl.obolibrary.org/obo/UO_0000111 -->

    <owl:Class rdf:about="http://purl.obolibrary.org/obo/UO_0000111">
        <rdfs:subClassOf rdf:resource="http://purl.obolibrary.org/obo/UO_0000000"/>
        <rdfs:comment>&quot;A unit which is a standard measure of the work done by a certain force (gravitational, electric, magnetic, force of inertia, etc).&quot; [NIST:NIST]</rdfs:comment>
        <rdfs:label>energy unit</rdfs:label>
    </owl:Class>
    


    <!-- http://purl.obolibrary.org/obo/UO_0000150 -->

    <owl:Class rdf:about="http://purl.obolibrary.org/obo/UO_0000150">
        <rdfs:subClassOf rdf:resource="http://purl.obolibrary.org/obo/UO_1000010"/>
        <oboInOwl:hasExactSynonym>ns</oboInOwl:hasExactSynonym>
        <rdfs:comment>&quot;A time unit which is equal to one thousandth of one millionth of a second or 10^[-9] s.&quot; [NIST:NIST]</rdfs:comment>
        <rdfs:label>nanosecond</rdfs:label>
    </owl:Class>
    


    <!-- http://purl.obolibrary.org/obo/UO_0000219 -->

    <owl:Class rdf:about="http://purl.obolibrary.org/obo/UO_0000219">
        <rdfs:subClassOf rdf:resource="http://purl.obolibrary.org/obo/UO_0000000"/>
        <rdfs:comment>&quot;A unit which is a standard measure of the quantity of unbalanced electricity in a body (either positive or negative) and construed as an excess or deficiency of electrons.&quot; [WordNet:WordNet]</rdfs:comment>
        <rdfs:label>electric charge</rdfs:label>
    </owl:Class>
    


    <!-- http://purl.obolibrary.org/obo/UO_0000221 -->

    <owl:Class rdf:about="http://purl.obolibrary.org/obo/UO_0000221">
        <rdfs:subClassOf rdf:resource="http://purl.obolibrary.org/obo/UO_1000221"/>
        <oboInOwl:hasExactSynonym>Da</oboInOwl:hasExactSynonym>
        <oboInOwl:hasExactSynonym>amu</oboInOwl:hasExactSynonym>
        <oboInOwl:hasExactSynonym>u</oboInOwl:hasExactSynonym>
        <oboInOwl:hasExactSynonym>unified atomic mass unit</oboInOwl:hasExactSynonym>
        <rdfs:comment>&quot;An independently to the base SI units defined mass unit which is equal to one twelfth of the mass of an unbound atom of the carbon-12 nuclide, at rest and in its ground state.&quot; [Wikipedia:Wikipedia]</rdfs:comment>
        <rdfs:label>dalton</rdfs:label>
    </owl:Class>
    


    <!-- http://purl.obolibrary.org/obo/UO_0000324 -->

    <owl:Class rdf:about="http://purl.obolibrary.org/obo/UO_0000324">
        <rdfs:subClassOf rdf:resource="http://purl.obolibrary.org/obo/UO_0000047"/>
        <oboInOwl:hasRelatedSynonym>A^[2]</oboInOwl:hasRelatedSynonym>
        <rdfs:comment>&quot;An area unit which is equal to an area enclosed by a square with sides each 1 angstrom long.&quot; [UOC:GVG]</rdfs:comment>
        <rdfs:label>square angstrom</rdfs:label>
    </owl:Class>
    


    <!-- http://purl.obolibrary.org/obo/UO_0000325 -->

    <owl:Class rdf:about="http://purl.obolibrary.org/obo/UO_0000325">
        <rdfs:subClassOf rdf:resource="http://purl.obolibrary.org/obo/UO_0000105"/>
        <oboInOwl:hasRelatedSynonym>mH</oboInOwl:hasRelatedSynonym>
        <oboInOwl:hasRelatedSynonym>megahertz</oboInOwl:hasRelatedSynonym>
        <rdfs:comment>&quot;A frequency unit which is equal to one million hertz or 10^[6] V.&quot; [UOC:GVG]</rdfs:comment>
        <rdfs:label>megaHertz</rdfs:label>
    </owl:Class>
    


    <!-- http://purl.obolibrary.org/obo/UO_1000010 -->

    <owl:Class rdf:about="http://purl.obolibrary.org/obo/UO_1000010">
        <rdfs:subClassOf rdf:resource="http://purl.obolibrary.org/obo/UO_0000003"/>
        <rdfs:label>second based unit</rdfs:label>
    </owl:Class>
    


    <!-- http://purl.obolibrary.org/obo/UO_1000019 -->

    <owl:Class rdf:about="http://purl.obolibrary.org/obo/UO_1000019">
        <rdfs:subClassOf rdf:resource="http://purl.obolibrary.org/obo/UO_0000001"/>
        <rdfs:label>angstrom based unit</rdfs:label>
    </owl:Class>
    


    <!-- http://purl.obolibrary.org/obo/UO_1000062 -->

    <owl:Class rdf:about="http://purl.obolibrary.org/obo/UO_1000062">
        <rdfs:subClassOf rdf:resource="http://purl.obolibrary.org/obo/UO_0000061"/>
        <rdfs:label>molar based unit</rdfs:label>
    </owl:Class>
    


    <!-- http://purl.obolibrary.org/obo/UO_1000094 -->

    <owl:Class rdf:about="http://purl.obolibrary.org/obo/UO_1000094">
        <rdfs:subClassOf rdf:resource="http://purl.obolibrary.org/obo/UO_0000060"/>
        <rdfs:label>meter per second based unit</rdfs:label>
    </owl:Class>
    


    <!-- http://purl.obolibrary.org/obo/UO_1000221 -->

    <owl:Class rdf:about="http://purl.obolibrary.org/obo/UO_1000221">
        <rdfs:subClassOf rdf:resource="http://purl.obolibrary.org/obo/UO_0000002"/>
        <rdfs:label>dalton based unit</rdfs:label>
    </owl:Class>
</rdf:RDF>



<!-- Generated by the OWL API (version 4.5.29) https://github.com/owlcs/owlapi -->

